Revise the previous discrepancies in dealing with EBCDIC characters

dafny/StreamProcessor.dfy
@@ -58,73 +58,37 @@ module StreamProcessorModule {
 
     function GetEBCDICChar(code: int): char
     {
+      // Reference 1: https://en.wikipedia.org/wiki/EBCDIC.
+      // Reference 2: https://www.ibm.com/docs/en/i/7.1.0?topic=sets-invariant-character-set
+      // The following covers the invariant character set ("invariant subset")
+      // in which "the code point assignments do not change from code page to code page."
       match code
-      case 0x40 => ' '
 
-      case 0x81 => 'a'
-      case 0x82 => 'b'
-      case 0x83 => 'c'
-      case 0x84 => 'd'
-      case 0x85 => 'e'
-      case 0x86 => 'f'
-      case 0x87 => 'g'
-      case 0x88 => 'h'
-      case 0x89 => 'i'
-      case 0x91 => 'j'
-      case 0x92 => 'k'
-      case 0x93 => 'l'
-      case 0x94 => 'm'
-      case 0x95 => 'n'
-      case 0x96 => 'o'
-      case 0x97 => 'p'
-      case 0x98 => 'q'
-      case 0x99 => 'r'
-      case 0xA2 => 's'
-      case 0xA3 => 't'
-      case 0xA4 => 'u'
-      case 0xA5 => 'v'
-      case 0xA6 => 'w'
-      case 0xA7 => 'x'
-      case 0xA8 => 'y'
-      case 0xA9 => 'z'
+      case 0x40 => ' ' case 0x4B => '.' case 0x4C => '<' case 0x4D => '('
+      case 0x4E => '+' case 0x50 => '&' case 0x5C => '*' case 0x5D => ')'
+      case 0x5E => ';' case 0x60 => '-' case 0x61 => '/' case 0x6B => ','
+      case 0x6C => '%' case 0x6D => '_' case 0x6E => '>' case 0x6F => '?'
+      case 0x7A => ':' case 0x7D => '\'' case 0x7E => '=' case 0x7F => '"'
 
-      case 0xC1 => 'A'
-      case 0xC2 => 'B'
-      case 0xC3 => 'C'
-      case 0xC4 => 'D'
-      case 0xC5 => 'E'
-      case 0xC6 => 'F'
-      case 0xC7 => 'G'
-      case 0xC8 => 'H'
-      case 0xC9 => 'I'
-      case 0xD1 => 'J'
-      case 0xD2 => 'K'
-      case 0xD3 => 'L'
-      case 0xD4 => 'M'
-      case 0xD5 => 'N'
-      case 0xD6 => 'O'
-      case 0xD7 => 'P'
-      case 0xD8 => 'Q'
-      case 0xD9 => 'R'
-      case 0xE2 => 'S'
-      case 0xE3 => 'T'
-      case 0xE4 => 'U'
-      case 0xE5 => 'V'
-      case 0xE6 => 'W'
-      case 0xE7 => 'X'
-      case 0xE8 => 'Y'
-      case 0xE9 => 'Z'
+      case 0x81 => 'a' case 0x82 => 'b' case 0x83 => 'c' case 0x84 => 'd'
+      case 0x85 => 'e' case 0x86 => 'f' case 0x87 => 'g' case 0x88 => 'h'
+      case 0x89 => 'i' case 0x91 => 'j' case 0x92 => 'k' case 0x93 => 'l'
+      case 0x94 => 'm' case 0x95 => 'n' case 0x96 => 'o' case 0x97 => 'p'
+      case 0x98 => 'q' case 0x99 => 'r' case 0xA2 => 's' case 0xA3 => 't'
+      case 0xA4 => 'u' case 0xA5 => 'v' case 0xA6 => 'w' case 0xA7 => 'x'
+      case 0xA8 => 'y' case 0xA9 => 'z'
 
-      case 0xF0 => '0'
-      case 0xF1 => '1'
-      case 0xF2 => '2'
-      case 0xF3 => '3'
-      case 0xF4 => '4'
-      case 0xF5 => '5'
-      case 0xF6 => '6'
-      case 0xF7 => '7'
-      case 0xF8 => '8'
-      case 0xF9 => '9'
+      case 0xC1 => 'A' case 0xC2 => 'B' case 0xC3 => 'C' case 0xC4 => 'D'
+      case 0xC5 => 'E' case 0xC6 => 'F' case 0xC7 => 'G' case 0xC8 => 'H'
+      case 0xC9 => 'I' case 0xD1 => 'J' case 0xD2 => 'K' case 0xD3 => 'L'
+      case 0xD4 => 'M' case 0xD5 => 'N' case 0xD6 => 'O' case 0xD7 => 'P'
+      case 0xD8 => 'Q' case 0xD9 => 'R' case 0xE2 => 'S' case 0xE3 => 'T'
+      case 0xE4 => 'U' case 0xE5 => 'V' case 0xE6 => 'W' case 0xE7 => 'X'
+      case 0xE8 => 'Y' case 0xE9 => 'Z'
+
+      case 0xF0 => '0' case 0xF1 => '1' case 0xF2 => '2' case 0xF3 => '3'
+      case 0xF4 => '4' case 0xF5 => '5' case 0xF6 => '6' case 0xF7 => '7'
+      case 0xF8 => '8' case 0xF9 => '9'
 
       case _ => '?'
     }
@@ -135,7 +99,7 @@ module StreamProcessorModule {
       ensures (mode == BINARY) ==> (stream_mode == BINARY)
       ensures (card_ended || !res.output_ready) ==> res.output_ready
       ensures (card_ended && mode == TEXT) ==> (res.output_char == '\n' && res.output_bytes == [])
-      ensures (card_ended && mode == BINARY) ==> (res.output_bytes == [0x0A as bv8] && res.output_char == '?')
+      ensures (card_ended && mode == BINARY) ==> (res.output_bytes == [0x15 as bv8] && res.output_char == '?')
       ensures (!card_ended && mode == TEXT) ==> (res.output_char == GetEBCDICChar(ColumnToInteger(column)) && res.output_bytes == [])
       ensures (!card_ended && mode == BINARY) ==> (res.output_char == '?' && res.output_bytes == ColumnToBytes(column))
     {
@@ -151,7 +115,7 @@ module StreamProcessorModule {
             output_bytes := [];
           case BINARY =>
             output_char := '?';
-            output_bytes := [0x0A as bv8];
+            output_bytes := [0x15 as bv8];
         }
       }
       else {
