dafny/StreamProcessorTests.dfy
@@ -5,7 +5,7 @@ module StreamProcessorTestsModule {
   import Utils = UtilitiesModule
   import SP = StreamProcessorModule
 
-  method {:test} Test_SP_ModeSwitch(sp: SP.StreamProcessor, column: Utils.arrayOfLength12<bool>)
+  method {:test} Test_SP_Mode_Switch(sp: SP.StreamProcessor, column: Utils.arrayOfLength12<bool>)
     modifies sp
   {
     var res1 := sp.HandleInput(SP.TEXT, column, false);
@@ -29,7 +29,7 @@ module StreamProcessorTestsModule {
     ensures sp.stream_mode == SP.BINARY
     ensures res.output_ready
     ensures res.output_char == '?'
-    ensures res.output_bytes == [0x0A as bv8]
+    ensures res.output_bytes == [0x15 as bv8]
   {
     res := sp.HandleInput(SP.BINARY, column, true);
   }
@@ -73,6 +73,32 @@ module StreamProcessorTestsModule {
   {
     // 0x40 = 0d64 -> 0b 0000 0100 0000 (padded to 12 bits).
     var column := Utils.SeqToArr12_bool([false, false, false, false, false, true, false, false, false, false, false, false]);
+    res := sp.HandleInput(SP.BINARY, column, false);
+    assert sp.stream_mode == SP.BINARY;
+    assert res.output_ready;
+    assert res.output_char == '?';
+    assert res.output_bytes == sp.ColumnToBytes(column);
+  }
+
+  method {:test} Test_SP_EBCDIC_char_newline_TEXT(sp: SP.StreamProcessor) returns (res: SP.HandleInputResult)
+    modifies sp
+    requires sp.stream_mode == SP.TEXT
+  {
+    // 0x15 = 0d21 -> 0b 0000 0001 0101 (padded to 12 bits).
+    var column := Utils.SeqToArr12_bool([false, false, false, false, false, false, false, true, false, true, false, true]);
+    res := sp.HandleInput(SP.TEXT, column, false);
+    assert sp.stream_mode == SP.TEXT;
+    assert res.output_ready;
+    assert res.output_char == sp.GetEBCDICChar(sp.ColumnToInteger(column));
+    assert res.output_bytes == [];
+  }
+
+  method {:test} Test_SP_EBCDIC_char_newline_BINARY(sp: SP.StreamProcessor) returns (res: SP.HandleInputResult)
+    modifies sp
+    requires sp.stream_mode == SP.BINARY
+  {
+    // 0x15 = 0d21 -> 0b 0000 0001 0101 (padded to 12 bits).
+    var column := Utils.SeqToArr12_bool([false, false, false, false, false, false, false, true, false, true, false, true]);
     res := sp.HandleInput(SP.BINARY, column, false);
     assert sp.stream_mode == SP.BINARY;
     assert res.output_ready;
